Redefine the logic interface to use bientailment as equivalence; update the model

src/MicroSail/Sep/Logic.v
@@ -4,97 +4,74 @@ Require Import FunctionalExtensionality.
 Require Import MicroSail.Syntax.
 Require Import MicroSail.Sep.Spec.
 
-(* Adopted from VST: https://github.com/PrincetonUniversity/VST/blob/master/msl/seplog.v *)
-Class NatDed (A: Type) := {
-  andp : A -> A -> A;
-  orp : A -> A -> A;
-  (* existential quantification *)
-  exp : forall {T : Type}, (T -> A) -> A;
-  (* universal quantification *)
-  allp : forall {T : Type}, (T -> A) -> A;
-  imp : A -> A -> A;
+(* Abstract logic interface, implemented as a Coq typeclasses
 
-  (* Prop embedding *)
-  prop : Prop -> A;
-  (* P ⊢ Q *)
-  derives : A -> A -> Prop;
+   Partially adopted from Gregory Malecha's PhD thesis (Chapter 7.1) and
+   VST https://github.com/PrincetonUniversity/VST/blob/master/msl/seplog.v
+*)
 
-  TT := prop True;
-  FF := prop False;
-}.
+Class ILogic (L : Type) :=
+{ lentails : L -> L -> Prop;
+  ltrue : L;
+  lfalse : L;
+  land : L -> L -> L;
+  lor : L -> L -> L;
+  limpl : L -> L -> L;
+  lprop: Prop -> L;
+  lex : forall {T : Type}, (T -> L) -> L;
+  lall : forall {T : Type}, (T -> L) -> L
+ }.
+
 
 Delimit Scope logic with logic.
 Local Open Scope logic.
-Notation "P '⊢' Q" := (derives P Q) (at level 80, no associativity) : logic_derives.
-Open Scope logic_derives.
+Notation "P '⊢' Q" := (lentails P Q) (at level 80, no associativity) : logic_entails.
+Open Scope logic_entails.
 Notation "'∃' x .. y , P " :=
-  (exp (fun x => .. (exp (fun y => P%logic)) ..)) (at level 65, x binder, y binder, right associativity) : logic.
+  (lex (fun x => .. (lex (fun y => P%logic)) ..)) (at level 65, x binder, y binder, right associativity) : logic.
 Notation "'∀' x .. y , P " :=
-  (allp (fun x => .. (allp (fun y => P%logic)) ..)) (at level 65, x binder, y binder, right associativity) : logic.
-Infix "∨" := orp (at level 50, left associativity) : logic.
-Infix "∧" := andp (at level 40, left associativity) : logic.
-Notation "P '-->' Q" := (imp P Q) (at level 55, right associativity) : logic.
-Notation "P '<-->' Q" := (andp (imp P Q) (imp Q P)) (at level 57, no associativity) : logic.
-Notation "'!!' e" := (prop e) (at level 25) : logic.
+  (lall (fun x => .. (lall (fun y => P%logic)) ..)) (at level 65, x binder, y binder, right associativity) : logic.
+Infix "∨" := lor (at level 50, left associativity) : logic.
+Infix "∧" := land (at level 40, left associativity) : logic.
+Notation "P '-->' Q" := (limpl P Q) (at level 55, right associativity) : logic.
+Notation "P '<-->' Q" := (land (limpl P Q) (limpl Q P))
+  (at level 57, no associativity) : logic.
+Notation "P ≅ Q" := ((P ⊢ Q) /\ (Q ⊢ P)) (at level 50, no associativity) : logic.
+Notation "'!!' e" := (lprop e) (at level 25) : logic.
 
-Class NatDedAxioms (A : Type) {ND : NatDed A} := {
-  (* pred_ext : forall P Q, P ⊢ Q -> Q ⊢ P -> *)
-  (*                   P = Q; *)
-  derives_refl : forall P, P ⊢ P;
-  derives_trans : forall P Q R, P ⊢ Q -> Q ⊢ R ->
-                           P ⊢ R;
-
-  andp_right :  forall X P Q, X ⊢ P -> X ⊢ Q ->
-                         X ⊢ P ∧ Q;
-  andp_left1 :  forall P Q R, P ⊢ R ->
-                         P ∧ Q ⊢ R;
-  andp_left2 :  forall P Q R, Q ⊢ R ->
-                         P ∧ Q ⊢ R;
-  orp_left : forall P Q R, P ⊢ R -> Q ⊢ R ->
-                      P ∨ Q ⊢ R;
-  orp_right1 : forall P Q R, P ⊢ Q ->
-                        P ⊢ Q ∨ R;
-  orp_right2 : forall P Q R, P ⊢ R ->
-                        P ⊢ Q ∨ R;
-  exp_right : forall {B : Set} (x : B) (P: A) (Q: B -> A), P ⊢ (Q x) ->
-                                                     P ⊢ (exp Q);
-  exp_left : forall {B : Set} (P : B -> A) (Q : A),
-       (forall x, (P x) ⊢ Q) -> (exp P) ⊢ Q;
-  allp_left : forall {B : Set} (P: B -> A) x Q, (P x) ⊢ Q -> (allp P) ⊢ Q;
-  allp_right : forall {B : Set} (P: A) (Q: B -> A),  (forall v, P ⊢ (Q v)) -> P ⊢ (allp Q);
-  imp_andp_adjoint : forall P Q R, P ∧ Q ⊢ R <-> P ⊢ (Q --> R);
-  (* prop_left: forall (P: Prop) Q, (P -> TT ⊢ Q) -> (prop P) ⊢ Q; *)
-  (* prop_right: forall (P: Prop) Q, P -> ⊢ Q (prop P); *)
-  (* prop_imp_prop_left: forall (P Q: Prop), derives (imp (prop P) (prop Q)) (prop (P -> Q)); *)
-  (* allp_prop_left: forall {B: Set} (P: B -> Prop), derives (allp (fun b => prop (P b))) (prop (forall b, P b)) *)
-(* not_prop_right: forall (P: A) (Q: Prop), (Q -> derives P FF) -> derives P (prop (not Q)) *)
+Class ILogicLaws (L : Type) (LL : ILogic L) :=
+{ entails_refl  : forall P, P ⊢ P;
+  entails_trans : forall P Q R, P ⊢ Q -> Q ⊢ R -> P ⊢ R;
+  land_right :  forall X P Q, X ⊢ P -> X ⊢ Q -> X ⊢ P ∧ Q;
+  land_left1 :  forall P Q R, P ⊢ R -> P ∧ Q ⊢ R;
+  land_left2 :  forall P Q R, Q ⊢ R -> P ∧ Q ⊢ R;
+  lor_left : forall P Q R, P ⊢ R -> Q ⊢ R -> P ∨ Q ⊢ R;
+  lor_right1 : forall P Q R, P ⊢ Q -> P ⊢ Q ∨ R;
+  lor_right2 : forall P Q R, P ⊢ R -> P ⊢ Q ∨ R;
+  lex_right  : forall {B : Type} (x : B) (P: L) (Q: B -> L), P ⊢ (Q x) -> P ⊢ (lex Q);
+  lex_left   : forall {B : Type} (P : B -> L) (Q : L), (forall x, (P x) ⊢ Q) -> (lex P) ⊢ Q;
+  lall_left  : forall {B : Type} (P: B -> L) x Q, (P x) ⊢ Q -> (lall P) ⊢ Q;
+  lall_right : forall {B : Type} (P: L) (Q: B -> L),  (forall v, P ⊢ (Q v)) -> P ⊢ (lall Q);
+  limpl_and_adjoint : forall P Q R, P ∧ Q ⊢ R <-> P ⊢ (Q --> R);
 }.
 
-Class SepLog (A : Type) := {
-  is_NatDed :> NatDed A;
-  emp : A;
-  sepcon : A -> A -> A;
-  wand : A -> A -> A;
-  (* (* Existential magic wand *) *)
-  (* ewand : A -> A -> A; *)
+Class ISepLogic (L : Type) := {
+  is_ILogic :> ILogic L;
+  emp : L;
+  sepcon : L -> L -> L;
+  wand : L -> L -> L;
 }.
 
 Notation "P '✱' Q" := (sepcon P Q) (at level 45, left associativity) : logic.
 Notation "P '-✱' Q" := (wand P Q) (at level 60, right associativity) : logic.
-(* Notation "P '-◯' Q" := (ewand P Q) (* Typeset with -\ci5 *) *)
-  (* (at level 60, right associativity) : logic. *)
 
-Class SepLogAxioms (A : Type) {SL : SepLog A} := {
-  is_NatDedAxioms :> NatDedAxioms A;
-  sepcon_assoc: forall (P Q R : A), (P ✱ Q) ✱ R = P ✱ (Q ✱ R);
-  sepcon_comm:  forall (P Q : A), P ✱ Q = Q ✱ P;
-  wand_sepcon_adjoint: forall (P Q R : A), (P ✱ Q ⊢ R) <-> (P ⊢ Q -✱ R);
-  sepcon_andp_prop: forall (P R : A) (Q : Prop), P ✱ (!!Q ∧ R) = !!Q ∧ (P ✱ R);
-  sepcon_derives: forall P P' Q Q' : A, P ⊢ P' -> Q ⊢ Q' -> P ✱ Q ⊢ P' ✱ Q';
-  (* ewand_sepcon: forall (P Q R : A),  (P ✱ Q) -◯ R = P -◯ (Q ✱ R); *)
-  (* ewand_TT_sepcon: forall (P Q R: A), (P ✱ Q) ∧ (R -◯ TT) ⊢ (P ∧ (R -◯ TT)) ✱ (Q ∧ (R -◯ TT)); *)
-  (* exclude_elsewhere: forall (P Q : A), P ✱ Q ⊢ (P ∧ (Q -◯ TT)) ✱ Q; *)
-  (* ewand_conflict: forall (P Q R : A), P ✱ Q ⊢ FF -> P ∧ (Q -◯ R) ⊢ FF *)
+Class ISepLogicLaws (L : Type) (SL : ISepLogic L) := {
+  is_ILogicLaws :> ILogicLaws L is_ILogic;
+  sepcon_assoc: forall (P Q R : L), ((P ✱ Q) ✱ R) ≅ (P ✱ (Q ✱ R));
+  sepcon_comm:  forall (P Q : L), P ✱ Q ≅ Q ✱ P;
+  wand_sepcon_adjoint: forall (P Q R : L), (P ✱ Q ⊢ R) <-> (P ⊢ Q -✱ R);
+  sepcon_andp_prop: forall (P R : L) (Q : Prop), P ✱ (!!Q ∧ R) ≅ !!Q ∧ (P ✱ R);
+  sepcon_entails: forall P P' Q Q' : L, P ⊢ P' -> Q ⊢ Q' -> P ✱ Q ⊢ P' ✱ Q';
 }.
 
 Module Type HeapKit
@@ -103,10 +80,10 @@ Module Type HeapKit
        (Import progkit : ProgramKit typekit termkit)
        (Import assertkit : AssertionKit typekit termkit progkit).
 
-  Class Heaplet (A : Type) := {
-    is_SepLog :> SepLog A;
-    pred : forall (p : 𝑷) (ts : Env Lit (𝑷_Ty p)), A;
-    ptsreg : forall {σ : Ty} (r : 𝑹𝑬𝑮 σ) (t : Lit σ),  A
+  Class Heaplet (L : Type) := {
+    is_ISepLogic :> ISepLogic L;
+    pred : forall (p : 𝑷) (ts : Env Lit (𝑷_Ty p)), L;
+    ptsreg : forall {σ : Ty} (r : 𝑹𝑬𝑮 σ) (t : Lit σ), L
   }.
 
 Notation "r '↦' t" := (ptsreg r t) (at level 30).
