src/MicroSail/Sep/Model/Disjoint.v
@@ -4,7 +4,7 @@ Require Import MicroSail.Syntax.
 Require Import MicroSail.Environment.
 Require Import MicroSail.Sep.Logic.
 Require Import MicroSail.Sep.Spec.
-Require Import MicroSail.Sep.Hoare.
+(* Require Import MicroSail.Sep.Hoare. *)
 
 (* Simple model (aka Logic Instance) using disjoint register-heaps *)
 
@@ -29,24 +29,27 @@ Module Disjoint
 
   Definition emp : Heap := fun _ _ => None.
 
-  Definition HProp (Γ : Ctx (𝑿 * Ty)) := LocalStore Γ -> Heap -> Prop.
+  Definition HProp : Type := Heap -> Prop.
 
-  Program Instance HProp_NatDed (Γ : Ctx (𝑿 * Ty)) : NatDed (HProp Γ) :=
-  { andp := (fun P Q => (fun δ γ => P δ γ /\ Q δ γ));
-    orp  := (fun P Q => (fun δ γ => P δ γ \/ Q δ γ));
+  Instance HProp_ILogic : ILogic HProp :=
+  { land := (fun P Q => (fun γ => P γ /\ Q γ));
+    lor  := (fun P Q => (fun γ => P γ \/ Q γ));
     (* existential quantification *)
-    exp := (fun {T : Type} (P : T -> HProp Γ) => (fun δ γ => exists x, P x δ γ));
+    lex := (fun {T : Type} (P : T -> HProp) => (fun γ => exists x, P x γ));
     (* universal quantification *)
-    allp := (fun {T : Type} (P : T -> HProp Γ) => (fun δ γ => forall x, P x δ γ));
-    imp := (fun P Q => (fun δ γ => P δ γ -> Q δ γ));
+    lall := (fun {T : Type} (P : T -> HProp) => (fun γ => forall x, P x γ));
+    limpl := (fun P Q => (fun γ => P γ -> Q γ));
 
     (* Prop embedding *)
-    prop := (fun (p : Prop) => (fun δ γ => p));
+    lprop := (fun (p : Prop) => (fun _ => p));
     (* P ⊢ Q *)
-    derives := (fun P Q => forall δ γ, P δ γ -> Q δ γ)
+    lentails := (fun P Q => forall γ, P γ -> Q γ);
+
+    ltrue := fun _ => True;
+    lfalse := fun _ => False
   }.
 
-  Program Instance HProp_NatDedAxioms (Γ : Ctx (𝑿 * Ty)) : @NatDedAxioms _ (HProp_NatDed Γ).
+  Program Instance HProp_ILogicLaws : @ILogicLaws HProp HProp_ILogic.
   Solve Obligations with firstorder.
 
   (* Check if two heaps are disjoint,
@@ -58,10 +61,10 @@ Module Disjoint
                                      | Some x => Some x
                                      end.
 
-  Program Instance HProp_SepLog (Γ : Ctx (𝑿 * Ty)) : SepLog (HProp Γ) :=
-  { emp := fun δ γ => forall σ r, γ σ r = None;
-    sepcon P Q := fun δ γ => exists γl γr, split γ γl γr /\ P δ γl /\ Q δ γr;
-    wand P Q := fun δ γl => forall γ γr, split γ γl γr -> P δ γr -> Q δ γ
+  Program Instance HProp_ISepLogic : ISepLogic HProp :=
+  { emp := fun γ => forall σ r, γ σ r = None;
+    sepcon P Q := fun γ => exists γl γr, split γ γl γr /\ P γl /\ Q γr;
+    wand P Q := fun γl => forall γ γr, split γ γl γr -> P γr -> Q γ
   }.
 
   (* Solve a heap partitioning goal of form 'split γ γl γr' *)
@@ -77,12 +80,15 @@ Module Disjoint
       | [ H : Some ?l1 = Some ?l2 |- _ ] => rewrite H
       | [ |- _ /\ _ ] => split
       | [ |- _ \/ _ ] => auto
-      end; cbn in *; try congruence.
+      end; cbn in *; try congruence; try eauto with seplogic.
 
-  Lemma split_comm {Γ : Ctx (𝑿 * Ty)} : forall γ γ1 γ2, split γ γ1 γ2 -> split γ γ2 γ1.
+  Create HintDb seplogic.
+
+  Lemma split_comm : forall γ γ1 γ2, split γ γ1 γ2 -> split γ γ2 γ1.
   Proof. heap_solve_split. Qed.
+  Hint Resolve split_comm : seplogic.
 
-  Lemma split_emp {Γ : Ctx (𝑿 * Ty)} : forall γ γ1, split γ emp γ1 <-> γ = γ1.
+  Lemma split_emp : forall γ γ1, split γ emp γ1 <-> γ = γ1.
   Proof.
     intros γ γ1.
     split.
@@ -91,6 +97,7 @@ Module Disjoint
       heap_solve_split.
     - heap_solve_split.
   Qed.
+  Hint Resolve split_emp : seplogic.
 
   Lemma split_assoc : forall γ γl γr γll γlr,
     split γ γl γr -> split γl γll γlr ->
@@ -103,62 +110,65 @@ Module Disjoint
                end).
     split; heap_solve_split.
   Qed.
+  Hint Resolve split_assoc : seplogic.
 
-  Lemma sepcon_comm_forward (Γ : Ctx (𝑿 * Ty)) : forall (P Q : HProp Γ),
-      forall δ γ, (P ✱ Q --> Q ✱ P) δ γ.
+  Lemma sepcon_comm : forall (P Q : HProp), P ✱ Q ≅ Q ✱ P.
   Proof.
-    intros P Q δ γ.
+    intros P Q.
     cbn.
-    intros.
-    destruct H as [γl [γr H]].
-    exists γr. exists γl.
-    destruct H as [H1 [H2 H3]].
     split.
-    - apply (@split_comm Γ _ _ _ H1).
-    - firstorder.
-  Qed.
+    - intros.
+      destruct H as [γl [γr H]].
+      exists γr. exists γl.
+      destruct H as [H1 [H2 H3]].
+      split.
+      + apply (@split_comm _ _ _ H1).
+      + firstorder.
+   - admit.
+  Abort.
 
-  Lemma sepcon_assoc_forward {Γ : Ctx (𝑿 * Ty)} : forall (P Q R : HProp Γ),
-    forall δ γ, ((P ✱ Q ✱ R) --> (P ✱ (Q ✱ R))) δ γ.
+  Lemma sepcon_assoc_forward : forall (P Q R : HProp), P ✱ Q ✱ R ≅ P ✱ (Q ✱ R).
   Proof.
-    intros P Q R δ γ.
     cbn.
-    intros H.
-    destruct H as [γl [γr [H_split_1 [H HR]]]].
-    destruct H as [γl' [γr' [H_split_2 [HP HQ]]]].
-    specialize (split_assoc γ γl γr γl' γr' H_split_1 H_split_2) as H_split_3.
-    inversion H_split_3 as [γcomp H_split_comp].
-    exists γl'. exists γcomp.
+    intros P Q R.
     split.
-    - apply H_split_comp.
-    - split.
-      + apply HP.
-      + exists γr'. exists γr.
-        intuition.
-  Qed.
+    - intros γ.
+      cbn.
+      intros H.
+      destruct H as [γl [γr [H_split_1 [H HR]]]].
+      destruct H as [γl' [γr' [H_split_2 [HP HQ]]]].
+      specialize (split_assoc γ γl γr γl' γr' H_split_1 H_split_2) as H_split_3.
+      inversion H_split_3 as [γcomp H_split_comp].
+      exists γl'. exists γcomp.
+      split.
+      * apply H_split_comp.
+      * split.
+        + apply HP.
+        + exists γr'. exists γr.
+          intuition.
+    - admit.
+  Abort.
 
-  Lemma wand_sepcon_adjoint {Γ : Ctx (𝑿 * Ty)} : forall (P Q R : HProp Γ),
+  Lemma wand_sepcon_adjoint : forall (P Q R : HProp),
       (P ✱ Q ⊢ R) <-> (P ⊢ Q -✱ R).
   Proof.
     intros P Q R.
     split.
     - intros H.
       cbn in *.
-      intros δ γl HP γ γr H_split HQ.
-      specialize (H δ γ).
+      intros γl HP γ γr H_split HQ.
+      specialize (H γ).
       apply H.
       exists γl. exists γr.
       intuition.
     - intros H.
       cbn in *.
-      intros δ γl H1.
+      intros γl H1.
       (* specialize (H δ γl). *)
       destruct H1 as [γll [γlr [H_split [HP HQ]]]].
-      exact (H δ γll HP γl γlr H_split HQ).
+      exact (H γll HP γl γlr H_split HQ).
   Qed.
 
-Lemma sepcon_andp_prop {Γ : Ctx (𝑿 * Ty)} : forall (P R : HProp Γ) (Q : Prop),
-      (P ✱ (!!Q ∧ R)) <-> (!!Q ∧ (P ✱ R)).
-
-
-  sepcon_entails: forall P P' Q Q' : A, P ⊢ P' -> Q ⊢ Q' -> P ✱ Q ⊢ P' ✱ Q';
+Lemma sepcon_andp_prop : forall (P R : HProp) (Q : Prop),
+      (P ✱ (!!Q ∧ R)) ≅ (!!Q ∧ (P ✱ R)).
+Abort.
